theories/simulation/slsls.v
@@ -1,0 +1,259 @@
+(** * SLSLS Separation Logic Stuttering Local Simulation *)
+(* not to be confused with SLS LS, the infamous Space Launch System - Launch System *)
+
+From iris Require Import bi bi.lib.fixpoint bi.updates.
+From iris.proofmode Require Import tactics.
+From simuliris Require Import simulation.language.
+
+Inductive head_step_rtc {Λ} P : expr Λ → state Λ → expr Λ → state Λ → Prop :=
+  | head_rtc_base e σ: head_step_rtc P e σ e σ
+  | head_rtc_step e1 e2 e3 σ1 σ2 σ3 : head_step P e1 σ1 e2 σ2 → head_step_rtc P e2 σ2 e3 σ3 → head_step_rtc P e1 σ1 e3 σ3.
+Hint Constructors head_step_rtc : core.
+
+Inductive head_step_tc {Λ} P : expr Λ → state Λ → expr Λ → state Λ → Prop :=
+  | head_tc_base e e' σ σ' : head_step_tc P e σ e' σ'
+  | head_tc_step e1 e2 e3 σ1 σ2 σ3 : head_step P e1 σ1 e2 σ2 → head_step_tc P e2 σ2 e3 σ3 → head_step_tc P e1 σ1 e3 σ3.
+Hint Constructors head_step_tc : core.
+
+Definition reach_stuck {Λ : language} (P : prog Λ) (e : expr Λ) (σ : state Λ) :=
+  ∃ e' σ', head_step_rtc P e σ e' σ' ∧ stuck P e' σ'.
+
+Class simul_lang (PROP : bi) (Λ : language) := {
+  (* state interpretation *)
+  state_interp : prog Λ → state Λ → prog Λ → state Λ → PROP;
+  (* value relation that restricts values passed to functions *)
+  val_rel : val Λ → val Λ → PROP;
+}.
+Hint Mode simul_lang + - : typeclass_instances.
+
+(** Typeclass for the simulation relation so we can use the definitions with
+   greatest+least fp (stuttering) or just greatest fp (no stuttering). *)
+Class Sim {PROP : bi} {Λ : language} (s : simul_lang PROP Λ) := sim : (val Λ → val Λ → PROP) → expr Λ → expr Λ → PROP.
+Hint Mode Sim + + - : typeclass_instances.
+
+(* discrete OFE instance for expr *)
+Definition exprO {Λ : language} := leibnizO (expr Λ).
+
+Section fix_lang.
+  Context {PROP : bi}.
+
+  Context {Λ : language}.
+  Context {s : simul_lang PROP Λ}.
+
+  Definition sim_expr {sim : Sim s} Φ e_t e_s := sim Φ e_s e_t.
+  Definition sim_ctx {sim : Sim s} Φ K_t K_s :=
+    (∀ v_t v_s, val_rel v_t v_s -∗ sim_expr Φ (fill K_t (of_val v_t)) (fill K_s (of_val v_s)))%I.
+
+  Implicit Types
+    (e_s e_t e: expr Λ)
+    (P_s P_t P: prog Λ)
+    (σ_s σ_t σ : state Λ).
+
+
+  Context {PROP_bupd : BiBUpd PROP}.
+  Context {PROP_affine : BiAffine PROP}.
+
+  Section stuttering.
+    (** Simulation relation with stuttering *)
+
+    Definition least_step (Φ : val Λ → val Λ → PROP) (greatest_rec : expr Λ → expr Λ → PROP) (e_s : exprO) (least_rec : exprO → PROP) :=
+      λ (e_t : exprO), (∀ P_t σ_t P_s σ_s, state_interp P_t σ_t P_s σ_s ∗ ¬ ⌜reach_stuck P_s e_s σ_s⌝ -∗ |==>
+        (* value case *)
+        (∃ v_t v_s σ_s', ⌜to_val e_t = Some v_t⌝ ∗ ⌜head_step_rtc P_s e_s σ_s (of_val v_s) σ_s'⌝ ∗ Φ v_t v_s)
+
+        ∨ (* step case *)
+        (⌜reducible P_t e_t σ_t⌝ ∗ ∀ e_t' σ_t', ⌜head_step P_t e_t σ_t e_t' σ_t'⌝ -∗ |==>
+          (* stuttering *)
+          (state_interp P_t σ_t' P_s σ_s ∗ least_rec e_t') ∨
+          (* take a step *)
+          (∃ e_s' σ_s', ⌜head_step_tc P_s e_s σ_s e_s' σ_s'⌝ ∗ state_interp P_t σ_t' P_s σ_s' ∗ greatest_rec e_s' e_t'))
+
+        ∨ (* call case *)
+        (∃ f K_t v_t K_s v_s σ_s', ⌜e_t = fill K_t (of_call f v_t)⌝ ∗
+          ⌜head_step_rtc P_s e_s σ_s (fill K_s (of_call f v_s)) σ_s'⌝ ∗
+          val_rel v_t v_s ∗ state_interp P_t σ_t P_s σ_s' ∗
+          (∀ v_t v_s, val_rel v_t v_s -∗ greatest_rec (fill K_s (of_val v_s)) (fill K_t (of_val v_t))))
+      )%I.
+
+    Lemma least_step_mon Φ l1 l2 g1 g2 e_s:
+      ⊢ <pers> (∀ e, l1 e -∗ l2 e)
+      → <pers> (∀ e_s e_t, g1 e_s e_t -∗ g2 e_s e_t)
+      → ∀ e, least_step Φ g1 e_s l1 e -∗ least_step Φ g2 e_s l2 e.
+    Proof.
+      iIntros "#H #H0" (e) "Hl". rewrite /least_step. iIntros (P_t σ_t P_s σ_s) "Ha".
+      iMod ("Hl" with "Ha") as "[Hval | [Hstep | Hcall]]"; iModIntro.
+      + iLeft. iApply "Hval".
+      + iRight; iLeft. iDestruct "Hstep" as "[Hred Hr]"; iFrame "Hred".
+        iIntros (e_t' σ_t') "Hstep". iMod ("Hr" with "Hstep") as "[Hstay | Hstep]"; iModIntro.
+        { iLeft. iDestruct "Hstay" as "[$ H1]". by iApply "H". }
+        iRight. iDestruct "Hstep" as (e_s' σ_s') "(H1& H2 &H3)".
+        iExists (e_s'), (σ_s'). iFrame. by iApply "H0".
+      + iRight; iRight. iDestruct "Hcall" as (f K_t v_t K_s v_s σ_s') "(H1& H2& H3& H4&H5)".
+        iExists (f), (K_t), (v_t), (K_s), (v_s), (σ_s'). iFrame.
+        iIntros (? ?) "H1". iApply "H0". by iApply "H5".
+    Qed.
+
+    Instance least_step_mono (Φ : val Λ → val Λ → PROP) (greatest_rec : exprO → exprO → PROP) (e_s : exprO) :
+      BiMonoPred (least_step Φ greatest_rec e_s).
+    Proof.
+      constructor.
+      - intros l1 l2. iIntros "H". iApply (least_step_mon Φ l1 l2 greatest_rec greatest_rec e_s with "H").
+        eauto.
+      - intros l Hne n e1 e2 Heq.
+        apply discrete_iff in Heq as ->. reflexivity. apply _.
+    Qed.
+
+    Definition least_def (Φ : val Λ → val Λ → PROP) (greatest_rec : exprO → exprO → PROP) (e_s : exprO) :=
+      bi_least_fixpoint (least_step Φ greatest_rec e_s).
+
+    Lemma least_def_unfold (Φ : val Λ → val Λ → PROP) (greatest_rec : exprO → exprO → PROP) (e_s : exprO) e_t:
+      least_def Φ greatest_rec e_s e_t ⊣⊢ least_step Φ greatest_rec e_s (least_def Φ greatest_rec e_s) e_t.
+    Proof. by rewrite /least_def least_fixpoint_unfold. Qed.
+
+    Definition greatest_step (Φ : val Λ → val Λ → PROP) (greatest_rec : exprO * exprO → PROP) '(e_s, e_t) :=
+      least_def Φ (uncurry greatest_rec) e_s e_t.
+
+    Instance greatest_step_proper Φ greatest_rec:
+      Proper ((≡) ==> (≡)) (greatest_step Φ greatest_rec).
+    Proof. solve_proper. Qed.
+
+    Lemma least_def_mon Φ g1 g2 e_s:
+      ⊢ <pers> (∀ p, g1 p -∗ g2 p) → ∀ e, least_def Φ (uncurry g1) e_s e -∗ least_def Φ (uncurry g2) e_s e.
+    Proof.
+      iIntros "#H".
+      rewrite /least_def.
+      iApply (least_fixpoint_ind (least_step Φ (uncurry g1) e_s) (bi_least_fixpoint (least_step Φ (uncurry g2) e_s))).
+      iModIntro. iIntros (e).
+      rewrite least_fixpoint_unfold. iIntros "H0". iApply (least_step_mon Φ _ _ (uncurry g1) (uncurry g2) e_s).
+      - eauto.
+      - iModIntro. iIntros (? ?). rewrite /uncurry. by iApply "H".
+      - iApply "H0".
+    Qed.
+
+    Instance greatest_step_mono (Φ : val Λ → val Λ → PROP) :
+      BiMonoPred (greatest_step Φ).
+    Proof.
+      constructor.
+    - intros g1 g2.
+      iIntros "#H" ([e_s e_t]) "Hg". rewrite /greatest_step. iApply least_def_mon; eauto.
+    - intros g Hne n [e_s e_t] [e_s' e_t'] Heq. apply discrete_iff in Heq as [-> ->].
+      reflexivity. apply _.
+    Qed.
+
+    Definition sim_def (Φ : val Λ → val Λ → PROP) :=
+      bi_greatest_fixpoint (greatest_step Φ).
+
+    Lemma sim_def_unfold Φ e_s e_t:
+      sim_def Φ (e_s, e_t) ⊣⊢ greatest_step Φ (sim_def Φ) (e_s, e_t).
+    Proof. by rewrite /sim_def greatest_fixpoint_unfold. Qed.
+
+    Lemma sim_def_least_def_unfold Φ e_s e_t :
+      sim_def Φ (e_s, e_t) ⊣⊢ least_def Φ (uncurry (sim_def Φ)) e_s e_t.
+    Proof. by rewrite sim_def_unfold. Qed.
+
+    Definition sim_aux Φ : seal (@sim_def Φ). by eexists. Qed.
+    Instance sim_stutter : Sim s. intros Φ. exact (uncurry (sim_aux Φ).(unseal)). Defined.
+    Definition sim_eq Φ : sim_stutter Φ = uncurry (@sim_def Φ). by rewrite <- (sim_aux Φ).(seal_eq). Defined.
+    Lemma sim_expr_unfold Φ e_t e_s:
+      sim_expr (sim:=sim_stutter) Φ e_t e_s ⊣⊢
+      (∀ P_t σ_t P_s σ_s, state_interp P_t σ_t P_s σ_s ∗ ¬ ⌜reach_stuck P_s e_s σ_s⌝ -∗ |==>
+        (* value case *)
+          (∃ v_t v_s σ_s', ⌜to_val e_t = Some v_t⌝ ∗ ⌜head_step_rtc P_s e_s σ_s (of_val v_s) σ_s'⌝ ∗ Φ v_t v_s)
+
+        ∨ (* step case *)
+        (⌜reducible P_t e_t σ_t⌝ ∗ ∀ e_t' σ_t', ⌜head_step P_t e_t σ_t e_t' σ_t'⌝ -∗ |==>
+          (state_interp P_t σ_t' P_s σ_s ∗ sim_expr (sim:=sim_stutter) Φ e_t' e_s) ∨
+          (∃ e_s' σ_s', ⌜head_step_tc P_s e_s σ_s e_s' σ_s'⌝ ∗ state_interp P_t σ_t' P_s σ_s' ∗
+          sim_expr (sim:=sim_stutter) Φ e_t' e_s'))
+
+        ∨ (* call case *)
+        (∃ f K_t v_t K_s v_s σ_s', ⌜e_t = fill K_t (of_call f v_t)⌝ ∗
+          ⌜head_step_rtc P_s e_s σ_s (fill K_s (of_call f v_s)) σ_s'⌝ ∗
+          val_rel v_t v_s ∗ state_interp P_t σ_t P_s σ_s' ∗
+          sim_ctx (sim:=sim_stutter) Φ K_t K_s)
+      )%I.
+    Proof.
+      rewrite /sim_ctx /sim_expr  !sim_eq /uncurry sim_def_unfold /greatest_step.
+      rewrite least_def_unfold /least_step.
+      by setoid_rewrite <-sim_def_least_def_unfold.
+    Qed.
+
+  End stuttering.
+
+  Section no_stuttering.
+    (** Simpler relation without stuttering using just a greatest fp. *)
+
+    Definition step_nostutter (Φ : val Λ → val Λ → PROP) (greatest_rec : exprO * exprO → PROP) : exprO * exprO → PROP:=
+      λ '(e_s, e_t), (∀ P_t σ_t P_s σ_s, state_interp P_t σ_t P_s σ_s ∗ ¬ ⌜reach_stuck P_s e_s σ_s⌝ -∗ |==>
+        (* value case *)
+        (∃ v_t v_s σ_s', ⌜to_val e_t = Some v_t⌝ ∗ ⌜head_step_rtc P_s e_s σ_s (of_val v_s) σ_s'⌝ ∗ Φ v_t v_s)
+
+        ∨ (* step case *)
+        (⌜reducible P_t e_t σ_t⌝ ∗ ∀ e_t' σ_t', ⌜head_step P_t e_t σ_t e_t' σ_t'⌝ -∗ |==>
+          ∃ e_s' σ_s', ⌜head_step_tc P_s e_s σ_s e_s' σ_s'⌝ ∗ state_interp P_t σ_t' P_s σ_s' ∗ greatest_rec (e_s', e_t'))
+
+        ∨ (* call case *)
+        (∃ f K_t v_t K_s v_s σ_s', ⌜e_t = fill K_t (of_call f v_t)⌝ ∗
+          ⌜head_step_rtc P_s e_s σ_s (fill K_s (of_call f v_s)) σ_s'⌝ ∗
+          val_rel v_t v_s ∗ state_interp P_t σ_t P_s σ_s' ∗
+          (∀ v_t v_s, val_rel v_t v_s -∗ greatest_rec (fill K_s (of_val v_s), fill K_t (of_val v_t))))
+      )%I.
+
+    Definition sim_nostutter_def (Φ : val Λ → val Λ → PROP) :=
+      bi_greatest_fixpoint (step_nostutter Φ).
+
+    Instance step_nostutter_proper Φ rec:
+      Proper ((≡) ==> (≡)) (step_nostutter Φ rec).
+    Proof. solve_proper. Qed.
+
+    Instance step_nostutter_mono (Φ : val Λ → val Λ → PROP):
+      BiMonoPred (step_nostutter Φ).
+    Proof.
+      constructor.
+      - intros g1 g2. iIntros "#H".
+        iIntros ([e_s e_t]) "Hg". rewrite /step_nostutter.
+        iIntros (P_t σ_t P_s σ_s) "Ha".
+        iMod ("Hg" with "Ha") as "[Hval | [Hstep | Hcall]]"; iModIntro.
+        + iLeft. iApply "Hval".
+        + iRight; iLeft. iDestruct "Hstep" as "[Hred Hr]"; iFrame "Hred".
+          iIntros (e_t' σ_t') "Hstep". iMod ("Hr" with "Hstep") as "Hstep"; iModIntro.
+          iDestruct "Hstep" as (e_s' σ_s') "(H1& H2 &H3)".
+          iExists (e_s'), (σ_s'). iFrame. by iApply "H".
+        + iRight; iRight. iDestruct "Hcall" as (f K_t v_t K_s v_s σ_s') "(H1& H2& H3& H4&H5)".
+          iExists (f), (K_t), (v_t), (K_s), (v_s), (σ_s'). iFrame.
+          iIntros (? ?) "H1". iApply "H". by iApply "H5".
+      - intros g Hne n e1 e2 Heq.
+        apply discrete_iff in Heq as ->. reflexivity. apply _.
+    Qed.
+
+    Lemma sim_nostutter_def_unfold Φ e_s e_t:
+      sim_nostutter_def Φ (e_s, e_t) ⊣⊢ step_nostutter Φ (sim_nostutter_def Φ) (e_s, e_t).
+    Proof. by rewrite /sim_nostutter_def greatest_fixpoint_unfold. Qed.
+
+    Definition sim_nostutter_aux Φ : seal (@sim_nostutter_def Φ). by eexists. Qed.
+    Instance sim_nostutter : Sim s. intros Φ. exact (uncurry (sim_nostutter_aux Φ).(unseal)). Defined.
+    Definition sim_nostutter_eq Φ : sim_nostutter Φ = uncurry (@sim_nostutter_def Φ).
+      by rewrite <- (sim_nostutter_aux Φ).(seal_eq). Defined.
+
+    Lemma sim_expr_unfold_nostutter Φ e_t e_s:
+      sim_expr (sim:=sim_nostutter) Φ e_t e_s ⊣⊢
+      (∀ P_t σ_t P_s σ_s, state_interp P_t σ_t P_s σ_s ∗ ¬ ⌜reach_stuck P_s e_s σ_s⌝ -∗ |==>
+        (* value case *)
+          (∃ v_t v_s σ_s', ⌜to_val e_t = Some v_t⌝ ∗ ⌜head_step_rtc P_s e_s σ_s (of_val v_s) σ_s'⌝ ∗ Φ v_t v_s)
+
+        ∨ (* step case *)
+        (⌜reducible P_t e_t σ_t⌝ ∗ ∀ e_t' σ_t', ⌜head_step P_t e_t σ_t e_t' σ_t'⌝ -∗ |==>
+          ∃ e_s' σ_s', ⌜head_step_tc P_s e_s σ_s e_s' σ_s'⌝ ∗ state_interp P_t σ_t' P_s σ_s' ∗
+          sim_expr (sim:=sim_nostutter) Φ e_t' e_s')
+
+        ∨ (* call case *)
+        (∃ f K_t v_t K_s v_s σ_s', ⌜e_t = fill K_t (of_call f v_t)⌝ ∗
+          ⌜head_step_rtc P_s e_s σ_s (fill K_s (of_call f v_s)) σ_s'⌝ ∗
+          val_rel v_t v_s ∗ state_interp P_t σ_t P_s σ_s' ∗
+          sim_ctx (sim:=sim_nostutter) Φ K_t K_s)
+      )%I.
+    Proof.
+      by rewrite /sim_ctx /sim_expr !sim_nostutter_eq /uncurry sim_nostutter_def_unfold /step_nostutter.
+    Qed.
+  End no_stuttering.
+End fix_lang.
